better support for interfaces ... in progress

lib/seq.fsi
@@ -19,75 +19,81 @@ module Seq
 type seq : Type -> Type
 
 (* Destructors *)
-assume val length: a:Type -> seq a -> Tot nat
-assume val index:  a:Type -> s:seq a -> i:nat{i < length s} -> Tot a
+val length: a:Type -> seq a -> Tot nat
+val index:  a:Type -> s:seq a -> i:nat{i < length s} -> Tot a
 
 (* Constructors *)
-assume val create: a:Type -> nat -> a -> Tot (seq a)
-assume val upd:    a:Type -> s:seq a -> n:nat{n < length s} -> a ->  Tot (seq a)
-assume val append: a:Type -> seq a -> seq a -> Tot (seq a)
-assume val slice:  a:Type -> s:seq a -> i:nat -> j:nat{i <= j && j <= length s} -> Tot (seq a)
-
-(* The following lemmas, introduced to the SMT solver, 
-   allow reasoning about the primitives equationally. *)
+val create: a:Type -> nat -> a -> Tot (seq a)
+val upd:    a:Type -> s:seq a -> n:nat{n < length s} -> a ->  Tot (seq a)
+val append: a:Type -> seq a -> seq a -> Tot (seq a)
+val slice:  a:Type -> s:seq a -> i:nat -> j:nat{i <= j && j <= length s} -> Tot (seq a)
 
 (* Lemmas about length *)
-assume val lemma_create_len: a:Type -> n:nat -> i:a -> Lemma
+val lemma_create_len: a:Type -> n:nat -> i:a -> Lemma
   (requires True)
   (ensures (length (create n i) = n))
   [SMTPat (length (create n i))]
 
-assume val lemma_len_upd: a:Type -> n:nat -> v:a -> s:seq a{n < length s} -> Lemma
+val lemma_len_upd: a:Type -> n:nat -> v:a -> s:seq a{n < length s} -> Lemma
   (requires True)
   (ensures (length (upd s n v) = length s))
   [SMTPat (length (upd s n v))]
 
-assume val lemma_len_append: a:Type -> s1:seq a -> s2:seq a -> Lemma
+val lemma_len_append: a:Type -> s1:seq a -> s2:seq a -> Lemma
   (requires True)
   (ensures (length (append s1 s2) = length s1 + length s2))
   [SMTPat (length (append s1 s2))]
 
-assume val lemma_len_slice: a:Type -> s:seq a -> i:nat -> j:nat{i <= j && j <= length s} -> Lemma
+val lemma_len_slice: a:Type -> s:seq a -> i:nat -> j:nat{i <= j && j <= length s} -> Lemma
   (requires True)
   (ensures (length (slice s i j) = j - i))
   [SMTPat (length (slice s i j))]
 
 (* Lemmas about index *)
-assume val lemma_index_create: a:Type -> n:nat -> v:a -> i:nat{i < n} -> Lemma
+val lemma_index_create: a:Type -> n:nat -> v:a -> i:nat{i < n} -> Lemma
   (requires True)
   (ensures (index (create n v) i = v))
   [SMTPat (index (create n v) i)]
 
-assume val lemma_index_upd1: a:Type -> s:seq a -> n:nat{n < length s} -> v:a -> Lemma
+val lemma_index_upd1: a:Type -> s:seq a -> n:nat{n < length s} -> v:a -> Lemma
   (requires True)
   (ensures (index (upd s n v) n = v))
   [SMTPat (index (upd s n v) n)]
 
-assume val lemma_index_upd2: a:Type -> s:seq a -> n:nat{n < length s} -> v:a -> i:nat{i<>n /\ i < length s} -> Lemma
+val lemma_index_upd2: a:Type -> s:seq a -> n:nat{n < length s} -> v:a -> i:nat{i<>n /\ i < length s} -> Lemma
   (requires True)
   (ensures (index (upd s n v) i = index s i))
   [SMTPat (index (upd s n v) i)]
 
-assume val lemma_index_app1: a:Type -> s1:seq a -> s2:seq a -> i:nat{i < length s1} -> Lemma
+val lemma_index_app1: a:Type -> s1:seq a -> s2:seq a -> i:nat{i < length s1} -> Lemma
   (requires True)
   (ensures (index (append s1 s2) i = index s1 i))
   [SMTPat (index (append s1 s2) i)]
 
-assume val lemma_index_app2: a:Type -> s1:seq a -> s2:seq a -> i:nat{i < length s1 + length s2 /\ length s1 <= i} -> Lemma
+val lemma_index_app2: a:Type -> s1:seq a -> s2:seq a -> i:nat{i < length s1 + length s2 /\ length s1 <= i} -> Lemma
   (requires True)
   (ensures (index (append s1 s2) i = index s2 (i - length s1)))
   [SMTPat (index (append s1 s2) i)]
 
-assume val lemma_index_slice: a:Type -> s:seq a -> i:nat -> j:nat{i <= j /\ j <= length s} -> k:nat{k < j - i} -> Lemma
+val lemma_index_slice: a:Type -> s:seq a -> i:nat -> j:nat{i <= j /\ j <= length s} -> k:nat{k < j - i} -> Lemma
   (requires True)
   (ensures (index (slice s i j) k = index s (k + i)))
   [SMTPat (index (slice s i j) k)]
 
 (* Extensionality *)
-assume type Eq: #a:Type -> seq a -> seq a -> Type
-assume Equals:  forall (a:Type) (s1:seq a) (s2:seq a).{:pattern (Eq s1 s2)}             
-  Eq s1 s2 <==> 
-  (length s1 = length s2 /\
-  (forall (i:nat{i < length s1}).{:pattern (index s1 i); (index s2 i)} (index s1 i == index s2 i)))
-assume Extensional: forall (a:Type) (s1:seq a) (s2:seq a).{:pattern (Eq s1 s2)}             
-  Eq s1 s2 <==> s1==s2
+type Eq: #a:Type -> seq a -> seq a -> Type
+val lemma_eq_intro: a:Type -> s1:seq a -> s2:seq a -> Lemma
+     (requires (length s1 = length s2 
+               /\ (forall (i:nat{i < length s1}).{:pattern (index s1 i); (index s2 i)} (index s1 i == index s2 i))))
+     (ensures (Eq s1 s2))
+     [SMTPatT (Eq s1 s2)]
+
+val lemma_eq_refl: a:Type -> s1:seq a -> s2:seq a -> Lemma
+     (requires (s1 = s2))
+     (ensures (Eq s1 s2))
+     [SMTPatT (Eq s1 s2)]
+
+val lemma_eq_elim: a:Type -> s1:seq a -> s2:seq a -> Lemma
+     (requires (Eq s1 s2))
+     (ensures (s1=s2))
+     [SMTPatT (Eq s1 s2)]
