lib/set.fsi
@@ -1,0 +1,73 @@
+(*
+   Copyright 2008-2014 Nikhil Swamy, Aseem Rastogi, 
+                       Microsoft Research, University of Maryland
+
+   Licensed under the Apache License, Version 2.0 (the "License");
+   you may not use this file except in compliance with the License.
+   You may obtain a copy of the License at
+
+       http://www.apache.org/licenses/LICENSE-2.0
+
+   Unless required by applicable law or agreed to in writing, software
+   distributed under the License is distributed on an "AS IS" BASIS,
+   WITHOUT WARRANTIES OR CONDITIONS OF ANY KIND, either express or implied.
+   See the License for the specific language governing permissions and
+   limitations under the License.
+*)
+module Set
+
+type set : Type -> Type
+
+(* Destructors *)
+val mem : a:Type -> a -> set a -> Tot bool
+
+(* Constructors *)
+val empty      : a:Type -> Tot (set a)
+val singleton  : a:Type -> a -> Tot (set a)
+val union      : a:Type -> set a -> set a -> Tot (set a)
+val intersect  : a:Type -> set a -> set a -> Tot (set a)
+val complement : a:Type -> set a -> Tot (set a)
+
+(* Properties *)
+val mem_empty: a:Type -> x:a -> Lemma 
+   (requires True)
+   (ensures (not (mem x empty)))
+   [SMTPat (mem x empty)]                                           
+
+val mem_singleton: a:Type -> x:a -> Lemma 
+   (requires True)
+   (ensures (mem x (singleton x)))
+   [SMTPat (mem x (singleton x))]
+
+val mem_union: a:Type -> x:a -> s1:set a -> s2:set a -> Lemma 
+   (requires True)
+   (ensures (mem x (union s1 s2) = (mem x s1 || mem x s2)))
+   [SMTPat (mem x (union s1 s2))]
+
+val mem_intersect: a:Type -> x:a -> s1:set a -> s2:set a -> Lemma 
+   (requires True)
+   (ensures (mem x (intersect s1 s2) = (mem x s1 && mem x s2)))
+   [SMTPat (mem x (intersect s1 s2))]
+
+val mem_complement: a:Type -> x:a -> s:set a -> Lemma 
+   (requires True)
+   (ensures (mem x (complement s) = not(mem x s)))
+   [SMTPat (mem x (complement s))]
+
+(* Extensionality *)
+type Equal : #a:Type -> set a -> set a -> Type
+val lemma_equal_intro: a:Type -> s1:set a -> s2:set a -> Lemma 
+    (requires  (forall x. mem x s1 = mem x s2))
+    (ensures (Equal s1 s2))
+    [SMTPatT (Equal s1 s2)]
+
+val lemma_equal_elim: a:Type -> s1:set a -> s2:set a -> Lemma 
+    (requires (Equal s1 s2))
+    (ensures  (s1 = s2))
+    [SMTPatT (Equal s1 s2)]
+
+val lemma_equal_refl: a:Type -> s1:set a -> s2:set a -> Lemma 
+    (requires (s1 = s2))
+    (ensures  (Equal s1 s2))
+    [SMTPatT (Equal s1 s2)]
+
