examples/algorithms/qs_seq2.fst
@@ -1,29 +1,17 @@
 module QuickSort.Seq
 open Seq
 open SeqProperties
-open SeqPermutation
-
-val cons_perm: a:Type -> tl:seq a -> s:seq a{length s > 0} ->
-         Lemma (requires (permutation a tl (tail s)))
-               (ensures (permutation a (cons (head s) tl) s))
-let cons_perm tl s = Seq.lemma_tl (head s) tl
-
-(* Defining a new predicate symbol *)
-type total_order (a:Type) (f: (a -> a -> Tot bool)) =
-    (forall a. f a a)                                           (* reflexivity   *)
-    /\ (forall a1 a2. (f a1 a2 /\ a1<>a2)  <==> not (f a2 a1))  (* anti-symmetry *)
-    /\ (forall a1 a2 a3. f a1 a2 /\ f a2 a3 ==> f a1 a3)        (* transitivity  *)
 
 opaque val partition: f:('a -> 'a -> Tot bool){total_order 'a f}
-    -> s:seq 'a -> pivot:nat{pivot < s.length} -> back:nat{pivot <= back /\ back < s.length} ->
+    -> s:seq 'a -> pivot:nat{pivot < length s} -> back:nat{pivot <= back /\ back < length s} ->
        Pure (seq 'a * seq 'a)
-         (requires (forall (i:nat{i < s.length}).
+         (requires (forall (i:nat{i < length s}).
                                  ((i <= pivot ==> f (index s i) (index s pivot))
                                   /\ (back < i  ==> f (index s pivot) (index s i)))))
          (ensures (fun res ->
                      (fun lo hi p ->
-                         (lo.length + hi.length = s.length)
-                      /\ (hi.length > 0)
+                         (length lo + length hi = length s)
+                      /\ (length hi > 0)
                       /\ (index hi 0 = p)
                       /\ (forall x. (mem x hi ==> f p x)
                                  /\ (mem x lo ==> f x p)
@@ -36,7 +24,7 @@ let rec partition f s pivot back =
   if pivot=back
   then (lemma_count_slice s pivot;
         let lo = slice s 0 pivot in
-        let hi = slice s pivot s.length in
+        let hi = slice s pivot (length s) in
         lemma_mem_count lo (fun x -> f x (index s pivot));
         lemma_mem_count hi (f (index s pivot));
         (lo, hi))
@@ -54,10 +42,10 @@ let rec partition f s pivot back =
 val sort: f:('a -> 'a -> Tot bool){total_order 'a f}
        -> s1:seq 'a
        -> Tot (s2:seq 'a{sorted f s2 /\ permutation 'a s1 s2})
-              (decreases (s1.length))
+              (decreases (length s1))
 let rec sort f s =
-  if s.length <= 1 then s
-  else let lo, hi = partition f s 0 (s.length - 1) in
+  if length s <= 1 then s
+  else let lo, hi = partition f s 0 (length s - 1) in
        let pivot = head hi in
 
        let hi_tl = tail hi in
