lib/set.fst
@@ -1,55 +1,44 @@
+(*
+   Copyright 2008-2014 Nikhil Swamy, Aseem Rastogi, 
+                       Microsoft Research, University of Maryland
+
+   Licensed under the Apache License, Version 2.0 (the "License");
+   you may not use this file except in compliance with the License.
+   You may obtain a copy of the License at
+
+       http://www.apache.org/licenses/LICENSE-2.0
+
+   Unless required by applicable law or agreed to in writing, software
+   distributed under the License is distributed on an "AS IS" BASIS,
+   WITHOUT WARRANTIES OR CONDITIONS OF ANY KIND, either express or implied.
+   See the License for the specific language governing permissions and
+   limitations under the License.
+*)
 module Set
 open Prims.PURE
 
-(*private extensional*) type set (a:Type) = a -> Tot bool
+type set (a:Type) = a -> Tot bool
 
-assume type Equal : #a:Type -> set a -> set a -> Type
+(* destructors *)
+let mem x s = s x
 
-(* private *) assume EqualDef : (forall (a:Type) (s1:set a) (s2:set a). Equal s1 s2 <==> (forall x. s1 x = s2 x))
+(* constructors *)
+let empty           = fun _ -> false
+let singleton x     = fun y -> y = x
+let union s1 s2     = fun x -> s1 x || s2 x
+let intersect s1 s2 = fun x -> s1 x && s2 x
+let complement s    = fun x -> not (s x)
 
-(* private *) assume Extensionality : (forall (a:Type) (s1:set a) (s2:set a). Equal s1 s2 <==> s1 = s2)
+(* properties *)
+let mem_empty x           = ()
+let mem_singleton x       = ()
+let mem_union x s1 s2     = ()
+let mem_intersect x s1 s2 = ()
+let mem_complement x s    = ()
 
-val empty : a:Type -> Tot (set a)
-(* private *) let empty = (fun _ -> false)
-
-val singleton : a:Type -> a -> Tot (set a)
-(* private *) let singleton x = (fun y -> y = x)
-
-val union : a:Type -> set a -> set a -> Tot (set a)
-(* private *) let union s1 s2 = (fun x -> s1 x || s2 x)
-
-val intersect : a:Type -> set a -> set a -> Tot (set a)
-(* private *) let intersect s1 s2 = (fun x -> s1 x && s2 x)
-
-val complement : a:Type -> set a -> Tot (set a)
-(* private *) let complement s = (fun x -> not (s x))
-
-val mem : a:Type -> a -> set a -> Tot bool
-(* private *) let mem x s = s x
-
-val memEmpty : a:Type -> x:a -> Lemma (requires True) (ensures (not (mem x empty))) [SMTPat (mem x empty)]
-(* private *) let memEmpty (a:Type) (x:a) = ()
-
-val memSingleton : a:Type -> x:a -> y:a -> Lemma (requires True) (ensures (mem x (singleton y) == (x = y))) [SMTPat (mem x (singleton y))]
-(* private *) let memSingleton (a:Type) (x:a) (y:a) = ()
-
-val memUnion : a:Type -> s1:set a -> s2:set a -> x:a -> Lemma (requires True) (ensures (mem x (union s1 s2) = (mem x s1 || mem x s2))) [SMTPat (mem x (union s1 s2))]
-(* private *) let memUnion (a:Type) (s1:set a) (s2:set a) (x:a) = ()
-
-val memIntersect : a:Type -> s1:set a -> s2:set a -> x:a -> Lemma (requires True) (ensures (mem x (intersect s1 s2) = (mem x s1 && mem x s2))) [SMTPat (mem x (intersect s1 s2))]
-(* private *) let memIntersect (a:Type) (s1:set a) (s2:set a) (x:a) = ()
-
-val memComplement : a:Type -> s:set a -> x:a -> Lemma (requires True) (ensures (mem x (complement s) = not (mem x s))) [SMTPat (mem x (complement s))]
-(* private *) let memComplement (a:Type) (s:set a) (x:a) = ()
-
-val extensional : a:Type -> s1:set a -> s2:set a -> Lemma (requires True) (ensures (Equal s1 s2 <==> s1 = s2)) (* error: [SMTPat (Equal a s1 s2)] *)
-(* private *) let extensional (a:Type) (s1:set a) (s2:set a) = ()
-
-val equals : a:Type -> s1:set a -> s2:set a -> Lemma (requires True) (ensures (Equal s1 s2 <==> (forall x. (* error: {:pattern (mem x s1); (mem x s2)}*) mem x s1 = mem x s2))) (* error: [SMTPat (Equal a s1 s2)] *)
-(* private *) let equals (a:Type) (s1:set a) (s2:set a) = ()
-
-let minus (a:Type) (s1:set a) (s2:set a) = intersect s1 (complement s2)
-
-opaque type Subset' (a:Type) (s1:set a) (s2:set a) = (forall (x:a).{:pattern mem x s1} mem x s1 ==> mem x s2)
-
-type Subset : #a:Type -> set a -> set a -> Type = fun (a:Type) (s1:set a) (s2:set a) -> Subset' a s1 s2
+(* extensionality *)
+open FunctionalExtensionality
+type Equal : #a:Type -> set a -> set a -> Type = fun (a:Type) (s1:set a) (s2:set a) -> FEq s1 s2
+let lemma_equal_intro s1 s2 = ()
+let lemma_equal_elim s1 s2 = ()
+let lemma_equal_refl s1 s2 = ()
